Restructure and add initial comments to nonreg proof

Game/FormalLanguages/BasicDefinitions.lean
@@ -1,32 +1,36 @@
 import Mathlib.Data.Set.Basic
+import Mathlib.Data.Nat.Defs
+
+open Nat
 
 namespace Regular
 
-inductive Symbol where
-  | a
-  | b
-
-instance : DecidableEq Symbol :=
-  λ
-  | .a, .a
-  | .b, .b => isTrue rfl
-  | .a, .b
-  | .b, .a => isFalse (by intro h; contradiction)
+def ex_alphabet : Set Char := {'a', 'b', 'c'}
 
 inductive Word where
   | ε
-  | cons (s : Symbol) (w : Word)
+  | cons (s : Char) (w : Word)
 
-def w₁ := Word.cons .a (Word.cons .b .ε)
-def w₂ := Word.cons .b (Word.cons .b (Word.cons .a .ε))
+def w₁ := Word.cons 'a' (Word.cons 'b' .ε)
+def w₂ := Word.cons 'b' (Word.cons 'b' (Word.cons 'a' .ε))
 
 @[simp]
-def Word.count (w : Word) (s' : Symbol) : ℕ := match w with
+def Word.chars : (w : Word) → Set Char
+  | ε => ∅
+  | cons s w => {s} ∪ w.chars
+
+structure Language where
+  Alphabet : Set Char
+  Words : Set Word
+  word_constraint : ∀ word ∈ Words, word.chars ⊆ Alphabet
+
+@[simp]
+def Word.count (w : Word) (s' : Char) : ℕ := match w with
   | .ε => 0
   | .cons s w => if (s = s') then 1 + w.count s' else w.count s'
-#reduce w₂.count .b
+#reduce w₂.count 'b'
 
-theorem count_uneq (w u : Word) : (∃ (s : Symbol), w.count s ≠ u.count s) → w ≠ u := by
+theorem count_uneq (w u : Word) : (∃ (s : Char), w.count s ≠ u.count s) → w ≠ u := by
   aesop
 
 @[simp]
@@ -43,6 +47,7 @@ def Word.cat (x y : Word) : Word :=
  | .cons s x => .cons s (x.cat y)
 
 infixr:90 " ∘ " => Word.cat
+--#reduce w₁ ∘ w₂
 
 @[simp]
 lemma Word.cat_eps (w : Word) : w ∘ .ε = w := by
@@ -55,7 +60,7 @@ lemma Word.cat_assoc (x y z : Word) : (x ∘ y) ∘ z = x ∘ y ∘ z := by
   induction' x with s w ih <;> simp_all only [cat]
 
 @[simp]
-lemma Word.assoc_count {s : Symbol} (x y : Word) :
+lemma Word.cat_count {s : Char} (x y : Word) :
     (x ∘ y).count s = x.count s + y.count s := by
   induction' x with s' w ih
   · simp_all only [cat, count, Nat.zero_add]
@@ -67,10 +72,24 @@ lemma Word.assoc_count {s : Symbol} (x y : Word) :
     next h => simp_all only
 
 @[simp]
-lemma Word.assoc_count_zero {s : Symbol} (x y : Word) :
+lemma Word.cat_count_zero {s : Char} (x y : Word) :
     (x ∘ y).count s = 0 → x.count s = 0 ∧ y.count s = 0 := by
   intro hcatcount
-  apply And.intro <;> simp_all only [assoc_count, Nat.add_eq_zero_iff]
+  apply And.intro <;> simp_all only [cat_count, Nat.add_eq_zero_iff]
+
+@[simp]
+lemma Word.cat_chars (x y : Word) : (x ∘ y).chars = x.chars ∪ y.chars := by
+  induction' x with s w ih
+  · simp only [cat, chars, Set.empty_union]
+  · aesop
+
+lemma Word.cat_char_subset_left (x y : Word) :
+    x.chars ⊆ (x ∘ y).chars := by
+  simp only [cat_chars, Set.subset_union_left]
+
+lemma Word.cat_char_subset_right (x y : Word) :
+    y.chars ⊆ (x ∘ y).chars := by
+  simp only [cat_chars, Set.subset_union_right]
 
 lemma Word.cat_len (x y : Word) :
     |(x ∘ y)| = |x| + |y| := by
@@ -79,7 +98,6 @@ lemma Word.cat_len (x y : Word) :
   · rw [Word.length, Nat.add_assoc, ← ih]
     simp_all only [length]
 
-#reduce w₂ ∘ w₁ ∘ w₁
 @[simp]
 def Word.pow (w : Word) (n : ℕ) : Word :=
   match n with
@@ -91,15 +109,15 @@ infix:92 " ^ " => Word.pow
 --#reduce w₁ ^ 3
 
 @[simp]
-def Symbol.pow (a : Symbol) (n : ℕ) : Word :=
+def Symbol.pow (a : Char) (n : ℕ) : Word :=
   match n with
   | 0 => .ε
   | .succ n => .cons a (Symbol.pow a n)
 
 infix:91 " ^+^ " => Symbol.pow
-#reduce .a ^+^ 5 ∘ .b ^+^ 3
 
-lemma Symbol.pow_len {s : Symbol} (n : ℕ) : |s ^+^ n| = n := by
+@[simp]
+lemma Symbol.pow_len {s : Char} (n : ℕ) : |s ^+^ n| = n := by
   induction' n with n ih
   · rfl
   · simp only [pow, Word.length]
@@ -107,7 +125,13 @@ lemma Symbol.pow_len {s : Symbol} (n : ℕ) : |s ^+^ n| = n := by
     exact Nat.one_add _
 
 @[simp]
-lemma Symbol.pow_count {s₁ s₂ : Symbol} (n : ℕ) :
+lemma Symbol.pow_chars {s : Char} {n : ℕ} (hn : n > 0) : (s ^+^ n).chars = {s} := by
+  induction' n, hn using Nat.le_induction with n
+  · simp_all only [Word.chars, Set.union_empty]
+  · simp_all only [Word.chars, add_eq, Nat.add_zero, Set.union_self]
+
+@[simp]
+lemma Symbol.pow_count {s₁ s₂ : Char} (n : ℕ) :
     (s₁ ^+^ n).count s₂ = if s₁ = s₂ then n else 0 := by
   induction' n with n ih
   · simp_all only [pow, Word.count, ite_self]
@@ -119,132 +143,158 @@ lemma Symbol.pow_count {s₁ s₂ : Symbol} (n : ℕ) :
       omega
     next h => simp_all only [↓reduceIte]
 
-def anbn : Set Word := {w | ∃ n, w = .a ^+^ n ∘ .b ^+^ n}
+def anbn : Set Word := {w | ∃ n, w = 'a' ^+^ n ∘ 'b' ^+^ n}
+def anbn_lang : Language := ⟨{'a', 'b'}, anbn,
+  by
+    intro w hw c hc
+    rw [anbn] at hw
+    simp_all only [Set.mem_setOf_eq, Set.mem_insert_iff, Set.mem_singleton_iff, ↓Char.isValue]
+    rcases hw with ⟨n, hw⟩
+    have hchars : w.chars = ('a' ^+^ n ∘ 'b' ^+^ n).chars := by rw [hw]
+    simp only [↓Char.isValue, Word.cat_chars] at hchars
+    rw [hchars] at hc
+    simp at hc
+    match n with
+    | 0 =>
+      simp_all only [Word.cat, Symbol.pow, Word.chars, Set.union_self, Set.mem_empty_iff_false, or_self]
+    | n + 1 =>
+      have hpowa := @Symbol.pow_chars 'a' (n + 1) (by omega)
+      have hpowb := @Symbol.pow_chars 'b' (n + 1) (by omega)
+      rw [hpowa, hpowb] at hc
+      simp only [↓Char.isValue, Set.mem_singleton_iff] at hc
+      exact hc
+  ⟩
+
 set_option linter.unusedVariables false
 
 @[simp]
-def pumping_property (L : Set Word) :=
+def pumping_property (L : Language) :=
   ∃ (n : ℕ) (hpos : n > 0),
-  ∀ z ∈ L,
+  ∀ z ∈ L.Words,
   (hlen : z.length > n) →
     ∃ (u v w : Word),
       z = u ∘ v ∘ w ∧
       |u ∘ v| ≤ n ∧
       |v| ≥ 1 ∧
-      ∀ (i : ℕ), u ∘ v ^ i ∘ w ∈ L
+      ∀ (i : ℕ), u ∘ v ^ i ∘ w ∈ L.Words
 
--- TODO: REFACTOR
-lemma Word.cons_a (n : ℕ) (x y z : Word) (hz : x ∘ y = .a ^+^ n ∘ z) (hx : |x| ≤ n) :
-    x.count .b = 0 := by
+--set_option tactic.simp.trace true
+lemma Word.cons_a (n : ℕ) (x y z : Word) (hz : x ∘ y = 'a' ^+^ n ∘ z) (hx : |x| ≤ n) :
+    x.count 'b' = 0 := by
   induction' x with s w ih generalizing n
   · simp_all only [Word.length, Nat.zero_le, Word.count]
   · specialize ih (n - 1)
-    simp_all only [Word.cat, Word.length, Word.count]
-    split
-    next h =>
-      subst h
-      simp_all only [Nat.add_eq_zero_iff, Nat.succ_ne_self, false_and]
+    simp_all only [Word.cat, Word.length, Word.count, ↓Char.isValue]
+    have ha : s = 'a' := by
+      clear ih
       match n with
-      | 0 =>
-        subst hz
-        simp_all only [Nat.le_zero_eq, Nat.add_eq_zero_iff, Nat.succ_ne_self, false_and]
+      | 0 => simp_all only [cat, le_zero_eq, Nat.add_eq_zero, succ_ne_self, false_and]
       | n + 1 =>
-        simp_all only [Nat.succ_sub_succ_eq_sub, Nat.sub_zero, cat, Nat.add_eq, Nat.add_zero,
-          cons.injEq, false_and]
-    next h =>
-      have ha : s = Symbol.a := by
-        match s with
-        | .a => rfl
-        | .b => exact False.elim (h rfl)
-      subst ha
-      match n with
-      | 0 =>
-        subst hz
-        simp_all only [not_false_eq_true, Nat.le_zero_eq, cat, Nat.zero_sub]
-        generalize length w = n at *
-        omega
-      | n + 1 =>
-        simp only [Nat.add_one_sub_one] at ih
-        rw [Symbol.pow] at hz
-        simp_all only [not_false_eq_true, cat, cons.injEq, true_and, forall_true_left]
-        exact ih (by omega)
+        simp_all only [cat, add_eq, Nat.add_zero, cons.injEq]
+    simp_all only [↓Char.isValue, Char.reduceEq, ↓reduceIte]
+    subst ha
+    match n with
+    | 0 =>
+      subst hz
+      simp_all only [le_zero_eq, Nat.add_eq_zero, succ_ne_self, false_and]
+    | n + 1 =>
+      simp only [Nat.add_one_sub_one, ↓Char.isValue] at ih
+      rw [Symbol.pow] at hz
+      simp_all only [not_false_eq_true, cat, cons.injEq, true_and, forall_true_left, ↓Char.isValue]
+      exact ih (by omega)
 
-lemma not_pump : ¬pumping_property anbn := by
+lemma not_pump : ¬pumping_property anbn_lang := by
   rw [pumping_property]
-  push_neg
-  intro n hpos
-  let z : Word := (.a ^+^ n) ∘ (.b ^+^ n)
-  have hzinnonreg : z ∈ anbn := by
+  push_neg  -- push_neg first
+  intro n hpos -- introduce n, and the hypothesis that n > 0
+
+  let z : Word := ('a' ^+^ n) ∘ ('b' ^+^ n) -- we need to use a fitting word
+  -- we'll need to show that the word is actually an element of anbn
+  have hzinanbn : z ∈ anbn := by
     simp_all only [gt_iff_lt]
     rw [anbn]
     simp only [Set.mem_setOf_eq]
     use n
   use z
-  simp only [gt_iff_lt, ge_iff_le]
+  -- simp only [gt_iff_lt, ge_iff_le]
+  -- we now need to show every conjunct
   constructor
-  · exact hzinnonreg
-  · have heq : z = Symbol.a ^+^ n ∘ Symbol.b ^+^ n := rfl
+  · exact hzinanbn -- maybe only prove this lemma now
+  · -- we only need this 'have' because we don't have access to 'set' rather than let
+    have heq : z = 'a' ^+^ n ∘ 'b' ^+^ n := rfl
+    -- now we need to handle this inner conjunction
     constructor
-    · rw [anbn] at hzinnonreg
-      rw [heq]
-      rw [Word.cat_len]
-      clear hzinnonreg
-      repeat rw [Symbol.pow_len]
-      exact Nat.lt_add_of_pos_right hpos
-    · intro u v w hcons hlenlower hv
+    · -- showing that the length of z is actually greater than n - fairly trivial step
+      rw [heq, Word.cat_len, Symbol.pow_len, Symbol.pow_len]
+      omega
+    · -- main part of the proof!
+      intro u v w hcons hlenlower hv
       use 2
-      have honlyas : v.count .b = 0 := by
+      -- it's obvious that v doesn't contain any b's, but we have to show it!
+      have honlyas : v.count 'b' = 0 := by
         clear hv
         have hz : |z| = 2*n := by
           rw [heq, Word.cat_len, Symbol.pow_len, Symbol.pow_len]
           omega
-        simp_all only [gt_iff_lt, z]
-        have huv : (u ∘ v).count .b = 0 := by
+        simp_all only [gt_iff_lt, z, ↓Char.isValue]
+        have huv : (u ∘ v).count 'b' = 0 := by
           symm at hcons
           rw [← Word.cat_assoc] at hcons
-          apply Word.cons_a n (u ∘ v) w (.b ^+^ n) hcons hlenlower
-        exact (@Word.assoc_count_zero Symbol.b u v huv).right
-      have hatleastonea : v.count .a > 0 := by
-        clear hzinnonreg hlenlower hcons heq u w z hpos n
+          apply Word.cons_a n (u ∘ v) w ('b' ^+^ n) hcons hlenlower
+        exact (@Word.cat_count_zero 'b' u v huv).right
+      -- this is almost as obvious, but much more involved to show!
+      have hatleastonea : v.count 'a' > 0 := by
+        have hzcharsinab := anbn_lang.word_constraint z hzinanbn
+        simp only [anbn_lang, ↓Char.isValue] at hzcharsinab
+        -- since v is a subword of z, its characters will be a subset of z's
+        have hsub : v.chars ⊆ z.chars := by
+          have hleft := Word.cat_char_subset_left v w
+          have hright := Word.cat_char_subset_right u (v ∘ w)
+          rw [hcons]
+          intro c hc
+          exact hright (hleft hc)
+        -- since z's characters are 'a' and 'b'
+        have hvchars : v.chars ⊆ {'a', 'b'} := subset_trans hsub hzcharsinab
+        -- clearing a bunch of hypotheses that will only be a distraction otherwise
+        clear hzinanbn hlenlower hcons heq u w z hpos n hzcharsinab hsub
+        -- from here on out we need a fairly lengthy induction
         induction' v with s w ih
         · simp_all only [Word.length, Nat.le_zero_eq, Nat.succ_ne_self]
-        · simp_all only [gt_iff_lt, Word.length, Nat.le_add_right, Word.count]
-          generalize w.count Symbol.a = n at *
+        · simp_all only [gt_iff_lt, Word.length, Nat.le_add_right, Word.count, ↓Char.isValue]
+          generalize w.count 'a' = n at *
           split_ifs with hs
-          · subst hs
-            simp_all only [ite_false, forall_true_left]
-            have hsim : 1 ≤ 1 + n := by exact Nat.le_add_right 1 n
-            exact hsim
-          · split at honlyas
-            next h =>
-              subst h
-              simp_all only [Nat.add_eq_zero_iff, Nat.succ_ne_self, false_and]
-            next h =>
-              simp_all only [forall_const]
-              match s with
-              | .a => exact False.elim (hs rfl)
-              | .b => exact False.elim (h rfl)
+          · exact Nat.le_add_right 1 n
+          · have hsb : s = 'b' := by
+              -- once again clearing unnecessary hypotheses
+              clear ih honlyas n
+              rw [Word.chars] at hvchars
+              have hsab := (Set.union_subset_iff.mp hvchars).left
+              -- with the preparatory work done, simp_all can take care of the rest
+              simp_all only [Set.singleton_union, Set.singleton_subset_iff, Set.mem_insert_iff,
+                Set.mem_singleton_iff, false_or]
+            split_ifs at honlyas with h
+            · simp_all only [Nat.add_eq_zero_iff, Nat.succ_ne_self, false_and]
+            · simp_all only
+      -- now we can proceed with the rest of the proof
       intro hin
-      rw [anbn] at hin
-      simp only [Word.pow, Word.cat_eps, Set.mem_setOf_eq] at hin
-      --have h (w : Word) : w ∈ nonreg → w.count .a = w.count .b := sorry
-      simp_all only [gt_iff_lt, Word.cat_assoc, z]
-      have huneven : (u ∘ v ∘ v ∘ w).count .a ≠ (u ∘ v ∘ v ∘ w).count .b := by
-        simp only [Word.assoc_count, ne_eq, z]
-        apply Aesop.BuiltinRules.not_intro
+      simp only [Word.pow, Word.cat_eps, Set.mem_setOf_eq, anbn_lang] at hin
+      -- clearing a few unneeded hypotheses
+      simp_all only [gt_iff_lt, Word.cat_assoc, z, ↓Char.isValue]
+      clear hlenlower hzinanbn hv hpos z
+      rcases hin with ⟨m, hm⟩
+      have heven : (u ∘ v ∘ v ∘ w).count 'a' = (u ∘ v ∘ v ∘ w).count 'b' := by
+        clear hatleastonea honlyas hcons
+        simp_all only [Word.cat_count, Symbol.pow_count, ite_true, ite_false, Nat.add_zero, Nat.zero_add, Char.reduceEq]
+      have huneven : (u ∘ v ∘ v ∘ w).count 'a' ≠ (u ∘ v ∘ v ∘ w).count 'b' := by
+        simp only [Word.cat_count, ne_eq, ↓Char.isValue]
         intro heq
-        have hcount : (u ∘ v ∘ w).count .a = (u ∘ v ∘ w).count .b := by
+        have hcount : (u ∘ v ∘ w).count 'a' = (u ∘ v ∘ w).count 'b' := by
           rw [← hcons]
           clear hcons
-          simp_all only [Nat.zero_add, Word.assoc_count, Symbol.pow_count, ite_true, ite_false,
-            Nat.add_zero]
-        simp only [Word.assoc_count] at hcount
-        have hgoal : v.count .a = v.count .b := by
+          simp_all only [Nat.zero_add, Word.cat_count, Symbol.pow_count, ite_true, ite_false,
+            Nat.add_zero, Nat.add_zero, Nat.zero_add, Char.reduceEq]
+        simp only [Word.cat_count, ↓Char.isValue] at hcount
+        have hgoal : v.count 'a' = v.count 'b' := by
           omega
-        simp_all only [lt_self_iff_false, z]
-      rcases hin with ⟨m, hm⟩
-      have heven : (u ∘ v ∘ v ∘ w).count .a = (u ∘ v ∘ v ∘ w).count .b := by
-        clear huneven
-        simp_all only [Word.assoc_count, Symbol.pow_count, ite_true, ite_false, Nat.add_zero,
-          Nat.zero_add]
-      simp_all only [Word.assoc_count, ne_eq, z]
+        simp_all only [lt_self_iff_false]
+      exact huneven heven
