Game/Levels/Lemmas/L09_pow_count.lean
@@ -1,3 +1,4 @@
+import Game.Levels.Lemmas.L08_pow_len
 import Game.Metadata
 
 World "Lemmas"
