Game/Levels/NonregProofs/L02_Proof.lean
@@ -1,0 +1,126 @@
+import Game.Levels.Lemmas.L09_pow_count
+import Game.Metadata
+
+World "NonregProofs"
+Level 2
+
+Title "Proving the nonregularity of aⁿbⁿ"
+
+Introduction "We are finally ready to work through a proof that utilizes the pumping lemma!
+The proof on paper is as follows:
+-
+...
+-
+
+We will want to replicate the structure of the proof in Lean, but it will turn out
+that some of the steps are far more difficult to realize than on paper. Therefore,
+we will mostly guide you through each of the individual steps; you should therefore
+try to follow the instructions closely, as later steps might be contingent on earlier
+ones so that the proof state is in a fitting form.
+"
+
+namespace Regular
+
+Statement not_pump : ¬pumping_property anbn_lang := by
+  rw [pumping_property]
+  push_neg
+  intro n hpos
+  let z : Word := ('a' ^+^ n) ∘ ('b' ^+^ n)
+  have hzinanbn : z ∈ anbn := by
+    simp_all only [gt_iff_lt]
+    rw [anbn]
+    simp only [Set.mem_setOf_eq]
+    use n
+  use z
+  simp only [gt_iff_lt, ge_iff_le]
+  constructor
+  · exact hzinanbn
+  · have heq : z = 'a' ^+^ n ∘ 'b' ^+^ n := rfl
+    constructor
+    · rw [anbn] at hzinanbn
+      rw [heq, Word.cat_len]
+      clear hzinanbn
+      repeat rw [Symbol.pow_len]
+      exact Nat.lt_add_of_pos_right hpos
+    · intro u v w hcons hlenlower hv
+      use 2
+      have honlyas : v.count 'b' = 0 := by
+        clear hv
+        have hz : |z| = 2*n := by
+          rw [heq, Word.cat_len, Symbol.pow_len, Symbol.pow_len]
+          omega
+        simp_all only [gt_iff_lt, z, ↓Char.isValue]
+        have huv : (u ∘ v).count 'b' = 0 := by
+          symm at hcons
+          rw [← Word.cat_assoc] at hcons
+          apply Word.cons_a n (u ∘ v) w ('b' ^+^ n) hcons hlenlower
+        exact (@Word.cat_count_zero 'b' u v huv).right
+      have hatleastonea : v.count 'a' > 0 := by
+        have hthing := anbn_lang.word_constraint z hzinanbn
+        have hsub : v.chars ⊆ z.chars := by
+          have hleft := Word.cat_char_subset_left v w
+          have hright := Word.cat_char_subset_right u (v ∘ w)
+          rw [hcons]
+          exact fun _ hin ↦ hright (hleft hin)
+        have hvchars : v.chars ⊆ {'a', 'b'} := fun _ a_1 ↦ hthing (hsub a_1)
+        clear hzinanbn hlenlower hcons heq u w z hpos n hthing hsub
+        induction' v with s w ih
+        · simp_all only [Word.length, Nat.le_zero_eq, Nat.succ_ne_self]
+        · simp_all only [gt_iff_lt, Word.length, Nat.le_add_right, Word.count, ↓Char.isValue]
+          generalize w.count 'a' = n at *
+          split_ifs with hs
+          · subst hs
+            have hsim : 1 ≤ 1 + n := by exact Nat.le_add_right 1 n
+            exact hsim
+          · have hsb : s = 'b' := by
+              clear ih honlyas n
+              rw [Word.chars] at hvchars
+              have hsab := (Set.union_subset_iff.mp hvchars).left
+              simp_all only [Set.singleton_union, Set.singleton_subset_iff, Set.mem_insert_iff,
+                Set.mem_singleton_iff, false_or]
+            split at honlyas
+            next h =>
+              subst h
+              simp_all only [Nat.add_eq_zero_iff, Nat.succ_ne_self, false_and]
+            next h =>
+              simp_all only
+      intro hin
+      rw [anbn_lang] at hin
+      simp only [Word.pow, Word.cat_eps, Set.mem_setOf_eq] at hin
+      simp_all only [gt_iff_lt, Word.cat_assoc, z]
+      have huneven : (u ∘ v ∘ v ∘ w).count 'a' ≠ (u ∘ v ∘ v ∘ w).count 'b' := by
+        simp only [Word.cat_count, ne_eq, z]
+        apply Aesop.BuiltinRules.not_intro
+        intro heq
+        have hcount : (u ∘ v ∘ w).count 'a' = (u ∘ v ∘ w).count 'b' := by
+          rw [← hcons]
+          clear hcons
+          simp_all only [Nat.zero_add, Word.cat_count, Symbol.pow_count, ite_true, ite_false,
+            Nat.add_zero]
+          simp_all only [↓Char.isValue,
+            Char.reduceEq,
+            ↓reduceIte,
+            Nat.add_zero,
+            Nat.zero_add]
+        simp only [Word.cat_count] at hcount
+        have hgoal : v.count 'a' = v.count 'b' := by
+          omega
+        simp_all only [lt_self_iff_false, z]
+      rcases hin with ⟨m, hm⟩
+      have heven : (u ∘ v ∘ v ∘ w).count 'a' = (u ∘ v ∘ v ∘ w).count 'b' := by
+        clear huneven
+        simp_all only [Word.cat_count, Symbol.pow_count, ite_true, ite_false, Nat.add_zero,
+          Nat.zero_add]
+        simp_all only [↓Char.isValue,
+          Char.reduceEq,
+          ↓reduceIte,
+          Nat.add_zero,
+          Nat.zero_add]
+      simp_all only [Word.cat_count, ne_eq, z]
+
+Conclusion "This last message appears if the level is solved."
+
+/- Use these commands to add items to the game's inventory. -/
+
+-- NewTheorem Nat.add_comm Nat.add_assoc
+-- NewDefinition Nat Add Eq
